# U(I)
$$
U_A(I) = \sqrt{\dfrac{\sum{(I - I_n)}^2}{90}}
$$
$$
U_B(I) = \dfrac{0,001A}{\sqrt{3}}
$$
$$
U_C(I) = \sqrt{(U_A^2(I) + U_B^2(I))}
$$
# U(t)
$$
U_B(t) =U_C(t)=  \dfrac{1s}{\sqrt{3}}
$$

# U(m)
$$
U_B(m) = U_C(m)=  \dfrac{0,001g}{\sqrt{3}}
$$
# U(k)
$$
U(k) = \sqrt{(\dfrac{1}{It} * U_C(m_1))^2 +(-\dfrac{1}{It} * U_C(m_2))^2 + (-\dfrac{m_2-m_1}{tI^2} * U_C(I))^2 + (\dfrac{m_2 - m_1}{It^2} * U_C(t))^2}
$$
# U(F)
$$
U(F) = \sqrt{(\dfrac{-M}{2k^2} * U(k))^2}
$$
# k i F
$$
k=(3,4 ± 0,0086) * 10^{-4} \dfrac{g}{As}
$$
$$
F = 94355 ± 240 \dfrac{C}{mol}  
$$
$$
k=2, \alpha=95\%
$$
$$
k=3,2 * 10^{-4}\dfrac{g}{As}
$$
$$
F = 96485 \dfrac{C}{mol}
$$

